cp; case analysis in send

pulse/ulib/experimental/Steel.Channel.Simplex.fst
@@ -24,14 +24,18 @@ type chan_t = {
 
 let half : perm = Steel.Permissions.(half_permission full)
 
+let chan_inv_cond (c:chan_t) (vsend:chan_val) (vrecv:chan_val) =
+      (if vsend.chan_ctr = vrecv.chan_ctr
+      then pure (vsend == vrecv)
+      else pure (more vrecv.chan_prot /\ vsend.chan_prot == step vrecv.chan_prot vrecv.chan_msg))
+
+let chan_inv_recv (c:chan_t) (vsend:chan_val) =
+  h_exists (fun (vrecv:chan_val) ->
+      pts_to c.recv half vrecv `star` chan_inv_cond c vsend vrecv)
+
 let chan_inv (c:chan_t) : hprop =
   h_exists (fun (vsend:chan_val) ->
-  h_exists (fun (vrecv:chan_val) ->
-    pts_to c.send half vsend `star`
-    pts_to c.recv half vrecv `star`
-    (if vsend.chan_ctr = vrecv.chan_ctr
-     then pure (vsend == vrecv)
-     else pure (more vrecv.chan_prot /\ vsend.chan_prot == step vrecv.chan_prot vrecv.chan_msg))))
+    pts_to c.send half vsend `star` chan_inv_recv c vsend)
 
 noeq
 type chan = {
@@ -142,3 +146,87 @@ let new_chan (p:prot)
     rewrite_eq_squash recv ch.chan_chan.recv (fun r -> in_state ch.chan_chan.send p `star` in_state r p);
     h_assert (sender ch p `star` receiver ch p);
     return #chan #(fun ch -> (sender ch p `star` receiver ch p)) ch
+
+let send_pre (p:prot{more p}) (c:chan_t) (vs vr:chan_val) : hprop =
+  (pts_to c.send half vs `star`
+   pts_to c.recv half vr `star`
+   chan_inv_cond c vs vr `star`
+   in_state c.send p)
+
+let send_pre_split (p:prot{more p}) (c:chan_t) (vs vr:chan_val) (b:bool) : hprop =
+  (pts_to c.send half vs `star`
+   pts_to c.recv half vr `star`
+   (if b then pure (vs == vr) else  pure (more vr.chan_prot /\ vs.chan_prot == step vr.chan_prot vr.chan_msg)) `star`
+   in_state c.send p)
+
+
+let send_pre_available (p:prot{more p}) (c:chan_t) (vs vr:chan_val) : hprop =
+    (pts_to c.send half vs `star`
+     pts_to c.recv half vr `star`
+     pure (vs == vr) `star`
+     in_state c.send p)
+
+let send_pre_blocked (p:prot{more p}) (c:chan_t) (vs vr:chan_val) : hprop =
+    (pts_to c.send half vs `star`
+     pts_to c.recv half vr `star`
+     pure (more vr.chan_prot /\ vs.chan_prot == step vr.chan_prot vr.chan_msg) `star`
+     in_state c.send p)
+
+let send_cond (#p:prot{more p}) (c:chan) (x:msg_t p) (vs vr:chan_val)
+              (then_: (unit -> SteelT unit (send_pre_available p c.chan_chan vs vr) (fun _ -> sender c (step p x))))
+              (else_: (unit -> SteelT unit (send_pre_blocked p c.chan_chan vs vr) (fun _ -> sender c (step p x))))
+    : SteelT unit (send_pre p c.chan_chan vs vr) (fun _ -> sender c (step p x))
+    = let cc = c.chan_chan in
+      h_assert (send_pre p cc vs vr);
+      h_assert (send_pre_split p cc vs vr (vs.chan_ctr = vr.chan_ctr));
+      cond (vs.chan_ctr = vr.chan_ctr) (send_pre_split p cc vs vr) _ then_ else_
+
+assume
+val send_available(#p:prot{more p}) (c:chan) (x:msg_t p) (vs vr:chan_val) (_:unit)
+  : SteelT unit (send_pre_available p c.chan_chan vs vr) (fun _ -> sender c (step p x))
+
+assume
+val send_blocked (#p:prot{more p}) (c:chan) (x:msg_t p) (vs vr:chan_val)
+                 (loop:(unit ->SteelT unit (sender c p) (fun _ -> sender c (step p x))))
+                 (_:unit)
+  : SteelT unit (send_pre_blocked p c.chan_chan vs vr) (fun _ -> sender c (step p x))
+
+let assoc_l (p q r:hprop)
+  : SteelT unit (p `star` (q `star` r)) (fun _ -> (p `star` q) `star` r)
+  = h_admit #unit _ _
+
+let rec send (#p:prot{more p}) (cc:chan) (x:msg_t p)
+  : SteelT unit (sender cc p) (fun _ -> sender cc (step p x))
+  = let c : chan_t = cc.chan_chan in
+    let l : lock (chan_inv c) = cc.chan_lock in
+    h_assert (in_state c.send p);
+    h_intro_emp_l _;
+    let _ = frame (fun _ -> acquire l) _ in
+    h_assert (chan_inv c `star` in_state c.send p);
+    let vs = frame (fun _ -> read_refine (chan_inv_recv c) c.send) _ in
+    h_assert ((pts_to c.send half vs `star` chan_inv_recv c vs) `star` in_state c.send p);
+    frame (fun _ -> h_commute _ _) _;
+    assoc_r _ _ _;
+    h_assert (chan_inv_recv c vs `star` (pts_to c.send half vs `star` in_state c.send p));
+    let vr = frame (fun _ -> read_refine (chan_inv_cond c vs) c.recv) _ in
+    h_assert ((pts_to c.recv half vr `star` chan_inv_cond c vs vr) `star` (pts_to c.send half vs `star` in_state c.send p));
+    rearrange _ _ _ _;
+    frame (fun _ -> h_commute _ _) _;
+    assoc_l _ _ _;
+    h_assert (send_pre p c vs vr);
+    rewrite_eq_squash c cc.chan_chan (fun x -> send_pre p x vs vr);
+    h_assert (send_pre p cc.chan_chan vs vr);
+    send_cond #p cc x vs vr (send_available #p cc x vs vr)
+                            (send_blocked #p cc x vs vr (fun _ -> send cc x))
+
+let rec send (#p:prot{more p}) (c:chan) (x:msg_t p)
+ : Steel unit
+   (expects sender c p)
+   (provides fun _ -> sender c (step p x))
+ = acquire c.inv;
+   let _, _, n0 = !c.chan.send in
+   let _, _, n1 = !c.chan.recv in
+   if n0 == n1 //last send received
+   then (c.chan.send := (p, x, n0 + 1);
+         release c.inv)
+   else (release c.inv; send c x) //spin
